ex_meta1.v
@@ -4,6 +4,7 @@ Import Utf8_core.
 Import ILLVarInt.MILL. (* only this *)
 Import ILLVarInt.Tacs. (* only this *)
 Require Import unprove.
+Import FormulaOrdered.
 Import FormulaMultiSet. (* and this *)
 Require Import ILL_equiv.
 
@@ -12,151 +13,78 @@ Local Open Scope ILL_scope.
 Local Open Scope Emma.
 
 Inductive boolP : Prop := trueP | falseP.
-
-Program Fixpoint exists_oplus_on_formula (cont: forall (e1:env) (f1:formula) (h1: e1 ⊢ f1) (e2:env) (f2:formula) (h2: e2 ⊢ f2),boolP) (φl φr:formula)  (e:env) (f:formula) (h: e ⊢ f) {struct h}: boolP :=
-match h with
-  | Id _ _ p => falseP
-  | Impl_R _ p q x => exists_oplus_on_formula cont φl φr _ _ x
-  | Impl_L _ Δ Δ' p q r _ _ x x0 => if exists_oplus_on_formula cont φl φr _ _ x then trueP else exists_oplus_on_formula cont φl φr _ _ x0
-  | Times_R _ Δ p q _ _ x x0 => if exists_oplus_on_formula cont φl φr _ _ x then trueP else exists_oplus_on_formula cont φl φr _ _ x0
-  | Times_L _ p q r _ x => exists_oplus_on_formula cont φl φr _ _ x
-  | One_R _ _  => falseP
-  | One_L _ p _ x => exists_oplus_on_formula cont φl φr _ _ x
-  | And_R _ p q x x0 => if exists_oplus_on_formula cont φl φr _ _ x then trueP else exists_oplus_on_formula cont φl φr _ _ x0
-  | And_L_1 _ p q r _ x => exists_oplus_on_formula cont φl φr _ _ x
-  | And_L_2 _ p q r _ x => exists_oplus_on_formula cont φl φr _ _ x
-  | Oplus_L _ p q r _ x x0 =>
-    if FormulaOrdered.eq_dec p φl
-      then if FormulaOrdered.eq_dec q φr
-        then cont _ _  x _ _ x0
-        else if exists_oplus_on_formula cont φl φr _ _ x then trueP else exists_oplus_on_formula cont φl φr _ _ x0
-      else if exists_oplus_on_formula cont φl φr _ _ x then trueP else exists_oplus_on_formula cont φl φr _ _ x0
-  | Oplus_R_1 _ p q x => exists_oplus_on_formula cont φl φr _ _ x
-  | Oplus_R_2 _ p q x => exists_oplus_on_formula cont φl φr _ _ x
-  | T_ _ => falseP
-  | Zero_ _ p x => falseP
-  | Bang_D _ p q _ x => exists_oplus_on_formula cont φl φr _ _ x
-  | Bang_C _ p q _ x => exists_oplus_on_formula cont φl φr _ _ x
-  | Bang_W _ p q _ x => exists_oplus_on_formula cont φl φr _ _ x
-end.
-
-Program Fixpoint forall_impl_l_on_formula
-  (cont:forall (e1:env) (f1:formula) (h1: e1 ⊢ f1) (e2:env) (f2:formula) (h2: e2 ⊢ f2), boolP)
-  (φl φr:formula)  (e:env) (f:formula) (h: e ⊢ f) {struct h}: boolP :=
-match h with
-  | Id _ _ p => trueP
-  | Impl_R _ p q x => forall_impl_l_on_formula cont φl φr _ _ x
-  | Impl_L _ Δ Δ' p q r _ _ x x0 =>
-    if FormulaOrdered.eq_dec p φl
-      then if FormulaOrdered.eq_dec q φr
-        then cont _ _ x _ _ x0 (*if (cont _ _  x) then falseP else negb (cont _ _  x0) *)
-        else
-          if forall_impl_l_on_formula cont φl φr _ _ x
-            then forall_impl_l_on_formula cont φl φr _ _ x0
-            else falseP
-      else if forall_impl_l_on_formula cont φl φr _ _ x then forall_impl_l_on_formula cont φl φr _ _ x0 else falseP
-  | Times_R _ Δ p q _ _ x x0 => if forall_impl_l_on_formula cont φl φr _ _ x then forall_impl_l_on_formula cont φl φr _ _ x0 else falseP
-  | Times_L _ p q r _ x => forall_impl_l_on_formula cont φl φr _ _ x
-  | One_R _ _ => trueP
-  | One_L _ p _ x => forall_impl_l_on_formula cont φl φr _ _ x
-  | And_R _ p q x x0 => if forall_impl_l_on_formula cont φl φr _ _ x then forall_impl_l_on_formula cont φl φr _ _ x0 else falseP
-  | And_L_1 _ p q r _ x => forall_impl_l_on_formula cont φl φr _ _ x
-  | And_L_2 _ p q r _ x => forall_impl_l_on_formula cont φl φr _ _ x
-  | Oplus_L _ p q r _ x x0 => if forall_impl_l_on_formula cont φl φr _ _ x then forall_impl_l_on_formula cont φl φr _ _ x0 else falseP
-  | Oplus_R_1 _ p q x => forall_impl_l_on_formula cont φl φr _ _ x
-  | Oplus_R_2 _ p q x => forall_impl_l_on_formula cont φl φr _ _ x
-  | T_ _ => trueP
-  | Zero_ _ p x => trueP
-  | Bang_D _ p q _ x => forall_impl_l_on_formula cont φl φr _ _ x
-  | Bang_C _ p q _ x => forall_impl_l_on_formula cont φl φr _ _ x
-  | Bang_W _ p q _ x => forall_impl_l_on_formula cont φl φr _ _ x
-end.
 Definition orP (b1 b2:boolP) := if b1 then trueP else b2.
 Definition negP (b:boolP) := if b then falseP else trueP.
 
-Definition not_exists_oplus_on_formula lhs rhs (e1:env) (f1:formula) (h1: e1 ⊢ f1) (e2:env) (f2:formula) (h2: e2 ⊢ f2) :=
-  negP (orP (exists_oplus_on_formula (fun _ _ _ _ _ _ => trueP) lhs rhs _ _ h1) (exists_oplus_on_formula (fun _ _ _ _ _ _ => trueP) lhs rhs _ _ h2)).
+Module MetaProp1.
+  Definition pred:Type := forall (e1:env) (f1:formula) (h1: e1 ⊢ f1),boolP. (*no-indent*)
+  Definition Ptrue:pred := (fun {_ _} _ => trueP).
+  Section funs. 
+    Context (test:pred) (φl φr:formula).
+    Arguments test {e1} {f1} h1.
+    (* This function returns true if at least one node in the proof h contains a rule of the form:
 
-Eval vm_compute in (forall_impl_l_on_formula (not_exists_oplus_on_formula (G⊸1) (G⊸V)) R E _ _ originelle).
-Eval vm_compute in (forall_impl_l_on_formula (not_exists_oplus_on_formula 1 ((B ⊸ V) & (B ⊸ 1))) G 1 _ _ originelle).
+     ----------- ⊕r1     or:      ----------- ⊕r2
+       ⊢ φl ⊕ φr                    ⊢ φl ⊕ φr     
 
-Program Fixpoint exists_AtheseA_on_formula
-  (cont: forall (e1:env) (f1:formula) (h1: e1 ⊢ f1),boolP)
-  (φl φr:formula)  (e:env) (f:formula) (h: e ⊢ f) {struct h}: boolP :=
-match h with
-  | Oplus_R_1 _ p q x =>
-    if FormulaOrdered.eq_dec p φl
-      then if FormulaOrdered.eq_dec q φr
-        then cont _ _  x
-        else exists_AtheseA_on_formula cont φl φr _ _ x
-      else exists_AtheseA_on_formula cont φl φr _ _ x
-  | Oplus_R_2 _ q p x =>
-    if FormulaOrdered.eq_dec p φl
-      then if FormulaOrdered.eq_dec q φr
-        then cont _ _  x
-        else exists_AtheseA_on_formula cont φl φr _ _ x
-      else exists_AtheseA_on_formula cont φl φr _ _ x
-  | Id _ _ p => falseP
-  | Impl_R _ p q x => exists_AtheseA_on_formula cont φl φr _ _ x
-  | Impl_L _ Δ Δ' p q r _ _ x x0 => exists_AtheseA_on_formula cont φl φr _ _ x0
-  | Times_R _ Δ p q _ _ x x0 => if exists_AtheseA_on_formula cont φl φr _ _ x then trueP else exists_AtheseA_on_formula cont φl φr _ _ x0
-  | Times_L _ p q r _ x => exists_AtheseA_on_formula cont φl φr _ _ x
-  | One_R _ _ => falseP
-  | One_L _ p _ x => exists_AtheseA_on_formula cont φl φr _ _ x
-  | And_R _ p q x x0 => if exists_AtheseA_on_formula cont φl φr _ _ x then trueP else exists_AtheseA_on_formula cont φl φr _ _ x0
-  | And_L_1 _ p q r _ x => exists_AtheseA_on_formula cont φl φr _ _ x
-  | And_L_2 _ p q r _ x => exists_AtheseA_on_formula cont φl φr _ _ x
-  | Oplus_L _ p q r _ x x0 => if exists_AtheseA_on_formula cont φl φr _ _ x then trueP else exists_AtheseA_on_formula cont φl φr _ _ x0
-  | T_ _ => falseP
-  | Zero_ _ p x => falseP
-  | Bang_D _ p q _ x => exists_AtheseA_on_formula cont φl φr _ _ x
-  | Bang_C _ p q _ x => exists_AtheseA_on_formula cont φl φr _ _ x
-  | Bang_W _ p q _ x => exists_AtheseA_on_formula cont φl φr _ _ x
-end.
+   for which predicate test returns true. In practice we will use the
+   predicate that is always true because we just want to check the
+   *presence* of such a node (cf. exist_oplus below). *)
+    Program Fixpoint ex_subprf {e:env} {f:formula} (h: e ⊢ f) {struct h}: boolP :=
+      match h with
+      | Oplus_R_1 _ p q x =>
+          if p =φ?= φl then if q =φ?= φr then test x else  ex_subprf x
+          else  ex_subprf x
+      | Oplus_R_2 _ q p x =>
+          if p =φ?= φl then if q =φ?= φr then test x else  ex_subprf x
+          else  ex_subprf x
+      | Id _ _ p => falseP
+      | Impl_R _ p q x =>  ex_subprf x
+      | Impl_L _ Δ Δ' p q r _ _ x x0 =>  ex_subprf x0
+      | Times_R _ Δ p q _ _ x x0 =>  orP ( ex_subprf x) ( ex_subprf x0)
+      | Times_L _ p q r _ x =>  ex_subprf x
+      | One_R _ _ => falseP
+      | One_L _ p _ x =>  ex_subprf x
+      | And_R _ p q x x0 => orP ( ex_subprf x) ( ex_subprf x0)
+      | And_L_1 _ p q r _ x =>  ex_subprf x
+      | And_L_2 _ p q r _ x =>  ex_subprf x
+      | Oplus_L _ p q r _ x x0 => orP ( ex_subprf x) ( ex_subprf x0)
+      | T_ _ => falseP
+      | Zero_ _ p x => falseP
+      | Bang_D _ p q _ x =>  ex_subprf x
+      | Bang_C _ p q _ x =>  ex_subprf x
+      | Bang_W _ p q _ x =>  ex_subprf x
+      end.
 
+  End funs.
+  Eval vm_compute in  ex_subprf Ptrue A M originelle.
+  Eval vm_compute in  ex_subprf Ptrue A M simpl_ex.
 
-Eval vm_compute in exists_AtheseA_on_formula (fun _ _ _ => trueP) A M _ _ originelle.
-Eval vm_compute in exists_AtheseA_on_formula (fun _ _ _ => trueP) A M _ _ simpl_ex.
+End MetaProp1.
+Include MetaProp1.
 
-Lemma exists_AtheseA_on_formula_proof_eq_compat :
-  ∀ f1 f2 Γ Γ' φ (h1:Γ⊢φ) (h2:Γ'⊢φ),
-  Proof_eq.eq h1 h2 ->
-    exists_AtheseA_on_formula (fun _ _ _ => trueP) f1 f2 _ _ h1
-    = exists_AtheseA_on_formula (fun _ _ _ => trueP) f1 f2 _ _ h2.
+Definition exist_oplus :=  ex_subprf Ptrue.
+Arguments exist_oplus φl φr {e f} h.
+
+Lemma  ex_subprf_proof_eq_compat : ∀ f1 f2 Γ Γ' φ (h1:Γ⊢φ) (h2:Γ'⊢φ),
+    h1 ≡≡ h2 ->
+    exist_oplus f1 f2 h1 = exist_oplus f1 f2 h2.
 Proof.
   intros f1 f2 Γ Γ' φ h1 h2 H.
-  induction H;simpl.
-  - reflexivity.
-  - auto.
-  - apply IHeq2.
-  - rewrite IHeq1;rewrite IHeq2;reflexivity.
-  - rewrite IHeq;reflexivity.
-  - reflexivity.
-  - rewrite IHeq;reflexivity.
-  - rewrite IHeq1;rewrite IHeq2;reflexivity.
-  - rewrite IHeq;reflexivity.
-  - rewrite IHeq;reflexivity.
-  - rewrite IHeq1;rewrite IHeq2;reflexivity.
-  - rewrite IHeq;reflexivity.
-  - rewrite IHeq;reflexivity.
-  - reflexivity.
-  - reflexivity.
-  - rewrite IHeq;reflexivity.
-  - rewrite IHeq;reflexivity.
-  - rewrite IHeq;reflexivity.
+  induction H;simpl;repeat progress match goal with
+                                      H: exist_oplus _ _ _ = _ |- _ => rewrite H
+                                    end;auto.
 Qed.
 
-Lemma exists_AtheseA_on_formula_proof_eq_pre_morph_compat :
+Lemma  ex_subprf_proof_eq_pre_morph_compat :
   ∀ f1 f2 Γ Γ' φ (h1:Γ⊢φ) (h2:Γ==Γ'),
-  exists_AtheseA_on_formula (fun _ _ _ => trueP) f1 f2 _ _ h1
-  = exists_AtheseA_on_formula (fun _ _ _ => trueP) f1 f2 _ _ (ILL_proof_pre_morph φ Γ Γ' h2 h1).
+    exist_oplus f1 f2 h1
+    = exist_oplus f1 f2 (ILL_proof_pre_morph φ Γ Γ' h2 h1).
 Proof.
   intros f1 f2 Γ Γ' φ h1 h2.
-  apply exists_AtheseA_on_formula_proof_eq_compat.
+  apply  ex_subprf_proof_eq_compat.
   apply Proof_eq.sym;apply Proof_eq.eq_pre_morph.
 Qed.
-
-
 
 Lemma simple: { G, ((B⊸S)&(B⊸R))&1,(G⊸B)⊕(G⊸S)} ⊢ S⊕R.
 Proof with try solve [ apply Id;reflexivity | prove_multiset_eq].
@@ -168,11 +96,11 @@ Proof with try solve [ apply Id;reflexivity | prove_multiset_eq].
   weak_impl_l B S...
   apply Oplus_R_1...
 
-(*
+  (*
   and_l_2 (B ⊸ S) (B ⊸ R).
   weak_impl_l B R...
   apply Oplus_R_2...
-*)
+   *)
 
   weak_impl_l G S...
   and_l_2 ((B ⊸ S) & (B ⊸ R)) 1.
@@ -181,34 +109,34 @@ Proof with try solve [ apply Id;reflexivity | prove_multiset_eq].
 Defined.
 
 
-Eval vm_compute in exists_AtheseA_on_formula (fun _ _ _ => trueP) A M _ _ originelle.
-Eval vm_compute in exists_AtheseA_on_formula (fun _ _ _ => trueP) S R _ _ originelle.
-Eval vm_compute in (exists_AtheseA_on_formula (fun _ _ _ => trueP) S R _ _ simple).
-Eval vm_compute in (exists_AtheseA_on_formula (fun _ _ _ => trueP) R S _ _ simple).
+Eval vm_compute in exist_oplus A M originelle.
+Eval vm_compute in exist_oplus S R originelle.
+Eval vm_compute in (exist_oplus S R simple).
+Eval vm_compute in (exist_oplus R S simple).
 
-Definition all_proofs_of env gamma := (forall (p:env⊢gamma), exists_AtheseA_on_formula (fun _ _ _ => trueP) S R _ _ p =trueP).
+Definition all_proofs_of env gamma := (forall (p:env⊢gamma), exist_oplus S R p =trueP).
 
 Definition no_proof_for env gamma := (forall (p:env⊢gamma), False).
 #[local] Hint Unfold all_proofs_of no_proof_for : proof.
 
 Lemma all_proofs_of_pre_morph : forall φ Γ Γ',
-  all_proofs_of Γ φ -> eq_bool Γ Γ' = true -> all_proofs_of Γ' φ.
+    all_proofs_of Γ φ -> eq_bool Γ Γ' = true -> all_proofs_of Γ' φ.
 Proof.
   unfold all_proofs_of.
   intros φ Γ Γ' Hall Heq p.
   apply eq_bool_correct in Heq.
-  assert (h:exists p': Γ⊢φ, Proof_eq.eq p p').
-    symmetry in Heq; exists (ILL_proof_pre_morph _ _ _ Heq p).
-    apply Proof_eq.sym;apply Proof_eq.eq_pre_morph.
-      destruct h as [p' h].
-      rewrite exists_AtheseA_on_formula_proof_eq_compat with (h2:=p') (1:=h); auto.
+  assert (h:exists p': Γ⊢φ, p ≡≡ p').
+  symmetry in Heq; exists (ILL_proof_pre_morph _ _ _ Heq p).
+  apply Proof_eq.sym;apply Proof_eq.eq_pre_morph.
+  destruct h as [p' h].
+  rewrite  ex_subprf_proof_eq_compat with (h2:=p') (1:=h); auto.
 Qed.
 #[local] Hint Resolve all_proofs_of_pre_morph : proof.
 
 
 Lemma all_proofs_of_pre_morph' :
   forall φ Γ Γ', all_proofs_of Γ φ -> eq_bool Γ Γ' = true ->
-    forall (p:Γ'⊢φ), exists_AtheseA_on_formula (fun _ _ _ => trueP) S R _ _ p =trueP.
+                 forall (p:Γ'⊢φ), exist_oplus S R p =trueP.
 Proof.
   intros φ Γ Γ' H H0 p.
   eapply all_proofs_of_pre_morph;eassumption.
@@ -217,7 +145,7 @@ Qed.
 #[local] Hint Rewrite all_proofs_of_pre_morph' : proof.
 Require Import Setoid.
 Add Morphism all_proofs_of with signature (eq ==> Logic.eq ==> iff) as
-all_proof_of_morph.
+      all_proof_of_morph.
 Proof.
   intros x y H y0.
   split;intros; eapply all_proofs_of_pre_morph;try eassumption.
@@ -235,64 +163,64 @@ Ltac clean p :=
 
 
 Ltac decompose_add :=
-    repeat (match goal with
-            | H : _ ∈ (_ :: _) |- _  =>
+  repeat (match goal with
+          | H : _ ∈ (_ :: _) |- _  =>
               destruct (mem_destruct _ _ _ H);clear H
-            | H : _ ∈ ∅ |- _ =>
+          | H : _ ∈ ∅ |- _ =>
               rewrite empty_no_mem in H;discriminate
-            | H : ILLVarInt.MILL.eq _ _ |- _ => apply eq_is_eq in H;subst
+          | H : ILLVarInt.MILL.eq _ _ |- _ => apply eq_is_eq in H;subst
           end).
 
 Ltac var_not_in_env_tac_simple n' H :=
-elim unusable_var_in_env with (n:=n') (1:=H);
-[
-  vm_compute;reflexivity |
-  vm_compute;reflexivity |
-  vm_compute;reflexivity |
-  vm_compute;reflexivity |
+  elim unusable_var_in_env with (n:=n') (1:=H);
+  [
+    vm_compute;reflexivity |
+    vm_compute;reflexivity |
+    vm_compute;reflexivity |
+    vm_compute;reflexivity |
     intros;decompose_add;simpl in *;repeat split;try discriminate;reflexivity
-].
+  ].
 
 Ltac var_not_in_env_tac_aux H env :=
   match env with
-    | Proposition ?n::?env' =>
+  | Proposition ?n::?env' =>
       (complete (var_not_in_env_tac_simple n H)) ||
-        var_not_in_env_tac_aux H env'
-    | _ :: ?env' =>  var_not_in_env_tac_aux H env'
+                                                 var_not_in_env_tac_aux H env'
+  | _ :: ?env' =>  var_not_in_env_tac_aux H env'
   end.
 
 Ltac var_not_in_env_tac H :=
   match type of H with
-    | ?env ⊢ _ =>
+  | ?env ⊢ _ =>
       var_not_in_env_tac_aux H env
   end.
 Ltac is_var_env gamma :=
   match gamma with
-    | empty => fail 1
-    | _ :: _ => fail 1
-    | _ \ _ => fail 1
-    | _ ∪ _ => fail 1
-    | _ => idtac
+  | empty => fail 1
+  | _ :: _ => fail 1
+  | _ \ _ => fail 1
+  | _ ∪ _ => fail 1
+  | _ => idtac
   end.
 
 
 Ltac finish :=
   simpl;try reflexivity;
-    try discriminate;
-    try (complete auto with proof);
-    try autorewrite with proof;
-      try (complete (apply False_ind;auto with proof));
-      match goal with
-        |- (if ?e then trueP else trueP ) = trueP =>
-          case e;reflexivity
-        | i:?e⊢Proposition ?n' |- _ =>
-          elim var_in_env with (n:=n') (3:=i);vm_compute;reflexivity
-        | H: ?env⊢?g |- _ =>
-          complete var_not_in_env_tac H
-        | H : ?s == ?t |- _ =>
-          (complete (apply eq_bool_complete in H;vm_compute in H;
-            discriminate))|| (progress repeat (rewrite H in * ))
-      end.
+  try discriminate;
+  try (complete auto with proof);
+  try autorewrite with proof;
+  try (complete (apply False_ind;auto with proof));
+  match goal with
+    |- (if ?e then trueP else trueP ) = trueP =>
+      case e;reflexivity
+  | i:?e⊢Proposition ?n' |- _ =>
+      elim var_in_env with (n:=n') (3:=i);vm_compute;reflexivity
+  | H: ?env⊢?g |- _ =>
+      complete var_not_in_env_tac H
+  | H : ?s == ?t |- _ =>
+      (complete (apply eq_bool_complete in H;vm_compute in H;
+                 discriminate))|| (progress repeat (rewrite H in * ))
+  end.
 
 Ltac decomp :=
   simpl;try reflexivity;
@@ -303,105 +231,105 @@ Ltac decomp :=
   | H : ?t = ?t |- _ => clear H
   | H : ?t == ?t |- _ => clear H
   | H:_ :: _ == _ ∪ _ |- _ =>
-    symmetry in H
+      symmetry in H
   | H: _ ∪ _ == _ :: _ |- _ =>
-    let delta := fresh "Δ" in
-    let h1 := fresh "H" in
-    let h2 := fresh "H" in
-    destruct (union_decompose _ _ _ _ H)
-      as [[delta [h1 h2]]|[delta [h1 h2]]];clear H
+      let delta := fresh "Δ" in
+      let h1 := fresh "H" in
+      let h2 := fresh "H" in
+      destruct (union_decompose _ _ _ _ H)
+        as [[delta [h1 h2]]|[delta [h1 h2]]];clear H
   | H: empty == _ ∪ _ |- _ =>
-    symmetry in H
+      symmetry in H
   | H: _ ∪ _ == empty |- _ =>
-    let h1 := fresh "H" in
-    let h2 := fresh "H" in
-    destruct (union_empty_decompose _ _  H) as [h1 h2];
-    clear H
+      let h1 := fresh "H" in
+      let h2 := fresh "H" in
+      destruct (union_empty_decompose _ _  H) as [h1 h2];
+      clear H
   | H : ?t == _ |- _ =>
-    is_var_env t;
-    match goal with
-    | H': context [t] |- _ =>
-      match H' with
-      | H => fail 1
-      | _ => fail 2
+      is_var_env t;
+      match goal with
+      | H': context [t] |- _ =>
+          match H' with
+          | H => fail 1
+          | _ => fail 2
+          end
+      | _ => clear H
       end
-    | _ => clear H
-    end
   | H: ILLVarInt.MILL.eq _ _ |- _ => apply eq_is_eq in H; try (injection H;clear H;intros;subst)
 
   | H: _ ∈ _ |- _ => complete (vm_compute in H;discriminate)
   | H: _ ∈ (add _ _) |- _ =>
-    destruct (mem_destruct _ _ _ H);clear H
+      destruct (mem_destruct _ _ _ H);clear H
   (* | H : ?s == ?t |- _ =>  *)
   (*   (complete (apply eq_bool_complete in H;vm_compute in H; *)
   (*     discriminate))|| (progress repeat (rewrite H in * )) *)
   | H : ?s == ?t |- _ =>
-    (progress repeat (rewrite H in * ))
+      (progress repeat (rewrite H in * ))
   | H: context C [ remove ?f ?env ] |- _ =>
-    match env with
-      context C' [ add f ?env' ] =>
-      let e := context C' [ env' ] in
-      setoid_replace (remove f env) with e in H by (apply eq_bool_correct;vm_compute;reflexivity)
-    end
-  | H:(?x ⊸ ?y) = _  |- _ =>
-    try discriminate H;injection H;clear H;intros;subst
-  | H: (_ ⊕ _) = _  |- _ =>
-    try discriminate H;injection H;clear H;intros;subst
-  | H:(_ ⊗ _) = _ |- _  =>
-    try discriminate H;injection H;clear H;intros;subst
-  | H: _  & _ = _  |- _  =>
-    try discriminate H;injection H;clear H;intros;subst
-  | H: _ = (?x ⊸ ?y) |- _ =>
-    try discriminate H;injection H;clear H;intros;subst
-  | H: _ = (_ ⊕ _) |- _ =>
-    try discriminate H;injection H;clear H;intros;subst
-  | H: _ = (_ ⊗ _) |- _  =>
-    try discriminate H;injection H;clear H;intros;subst
-  | H: _ = _  & _ |- _  =>
-    try discriminate H;injection H;clear H;intros;subst
-  | H: ?delta ⊢ _, H' : ?delta == ∅ |- _ =>
-    apply False_ind;rewrite H' in H;clear - H;clean H;finish
-  | H: ?env⊢?g |- _ =>
-    (* try complete var_not_in_env_tac H;  *)
-    match env with
-    | context C' [?env' \ ?f] =>
-      match env' with
-      | context C [add f ?env''] =>
-        let e' := context C [ env'' ] in
-        let e := context C' [ e' ] in
-        assert (heq: e == env) by (apply eq_bool_correct;vm_compute;reflexivity);
-        symmetry in heq;
-        let h := fresh "H" in
-        let i' := fresh "i" in
-        assert (h:(exists i':ILL_proof e g, Proof_eq.eq H i')) by (exists (ILL_proof_pre_morph _ _ _ heq H);
-                                                                          apply Proof_eq.sym;
-                                                                          apply Proof_eq.eq_pre_morph);
-        destruct h as [i' h];
-        rewrite exists_AtheseA_on_formula_proof_eq_compat with (h2:=i') (1:=h);
-        clear H h heq
+      match env with
+        context C' [ add f ?env' ] =>
+          let e := context C' [ env' ] in
+          setoid_replace (remove f env) with e in H by (apply eq_bool_correct;vm_compute;reflexivity)
       end
-    end
+  | H:(?x ⊸ ?y) = _  |- _ =>
+      try discriminate H;injection H;clear H;intros;subst
+  | H: (_ ⊕ _) = _  |- _ =>
+      try discriminate H;injection H;clear H;intros;subst
+  | H:(_ ⊗ _) = _ |- _  =>
+      try discriminate H;injection H;clear H;intros;subst
+  | H: _  & _ = _  |- _  =>
+      try discriminate H;injection H;clear H;intros;subst
+  | H: _ = (?x ⊸ ?y) |- _ =>
+      try discriminate H;injection H;clear H;intros;subst
+  | H: _ = (_ ⊕ _) |- _ =>
+      try discriminate H;injection H;clear H;intros;subst
+  | H: _ = (_ ⊗ _) |- _  =>
+      try discriminate H;injection H;clear H;intros;subst
+  | H: _ = _  & _ |- _  =>
+      try discriminate H;injection H;clear H;intros;subst
+  | H: ?delta ⊢ _, H' : ?delta == ∅ |- _ =>
+      apply False_ind;rewrite H' in H;clear - H;clean H;finish
+  | H: ?env⊢?g |- _ =>
+      (* try complete var_not_in_env_tac H;  *)
+      match env with
+      | context C' [?env' \ ?f] =>
+          match env' with
+          | context C [add f ?env''] =>
+              let e' := context C [ env'' ] in
+              let e := context C' [ e' ] in
+              assert (heq: e == env) by (apply eq_bool_correct;vm_compute;reflexivity);
+              symmetry in heq;
+              let h := fresh "H" in
+              let i' := fresh "i" in
+              assert (h:(exists i':ILL_proof e g, H ≡≡ i')) by (exists (ILL_proof_pre_morph _ _ _ heq H);
+                                                                       apply Proof_eq.sym;
+                                                                       apply Proof_eq.eq_pre_morph);
+              destruct h as [i' h];
+              rewrite  ex_subprf_proof_eq_compat with (h2:=i') (1:=h);
+              clear H h heq
+          end
+      end
   | H: ?t == ?t', i: ?env⊢?f |- _ =>
-    match env with
-    | context [ t ] =>
-      let f_env := (match eval pattern t in env with
-                    | ?f _ => f
-                    end) in
-      let env'0 := constr:(f_env t')  in
-      let env' := (eval cbv beta iota in env'0) in
-      let h := fresh "H" in
-      let i' := fresh "i" in
-      let heq := fresh "heq" in
-      assert (h:exists i': env'⊢f, Proof_eq.eq i i');[
-        assert (heq:env'==env) by (rewrite H;reflexivity);
-        symmetry in heq;
-        exists (ILL_proof_pre_morph _ _ _ heq i);
-        apply Proof_eq.sym;apply Proof_eq.eq_pre_morph
-      | destruct h as [i' h];
-        rewrite exists_AtheseA_on_formula_proof_eq_compat with (h2:=i') (1:=h);
-        clear i h;try (rewrite H in *;clear H)
-      ]
-    end
+      match env with
+      | context [ t ] =>
+          let f_env := (match eval pattern t in env with
+                        | ?f _ => f
+                        end) in
+          let env'0 := constr:(f_env t')  in
+          let env' := (eval cbv beta iota in env'0) in
+          let h := fresh "H" in
+          let i' := fresh "i" in
+          let heq := fresh "heq" in
+          assert (h:exists i': env'⊢f, i ≡≡ i');[
+              assert (heq:env'==env) by (rewrite H;reflexivity);
+              symmetry in heq;
+              exists (ILL_proof_pre_morph _ _ _ heq i);
+              apply Proof_eq.sym;apply Proof_eq.eq_pre_morph
+            | destruct h as [i' h];
+              rewrite  ex_subprf_proof_eq_compat with (h2:=i') (1:=h);
+              clear i h;try (rewrite H in *;clear H)
+            ]
+      end
   end.
 
 
@@ -410,23 +338,23 @@ Ltac one_step p := clean p; (repeat decomp);try (complete finish);auto with proo
 
 Ltac unusable_implies_tac n' f H :=
   apply unusable_implies with (1:=H) (n:=n') (φ:=f);
-    [
-      vm_compute;reflexivity |
-        vm_compute;reflexivity |
-          vm_compute;reflexivity |
-            intros;decompose_add;repeat split;simpl in *;try discriminate;reflexivity].
+  [
+    vm_compute;reflexivity |
+    vm_compute;reflexivity |
+    vm_compute;reflexivity |
+    intros;decompose_add;repeat split;simpl in *;try discriminate;reflexivity].
 
 Ltac unusable_var_strong_tac n1 n2 H :=
   apply unusable_var_in_env_strong with (1:=H) (n:=n1);[
-  vm_compute;reflexivity|
-  vm_compute;reflexivity|
-  vm_compute;reflexivity|
-  vm_compute;reflexivity|
-  intros;decompose_add;simpl in *;  repeat split;try discriminate;try reflexivity;auto;
-  intros _;right;
-  exists n2;
-    split;[((left;reflexivity)||(right;reflexivity))|split;[
-      intros;decompose_add;simpl;reflexivity|vm_compute;reflexivity]]].
+      vm_compute;reflexivity|
+      vm_compute;reflexivity|
+      vm_compute;reflexivity|
+      vm_compute;reflexivity|
+      intros;decompose_add;simpl in *;  repeat split;try discriminate;try reflexivity;auto;
+      intros _;right;
+      exists n2;
+      split;[((left;reflexivity)||(right;reflexivity))|split;[
+                intros;decompose_add;simpl;reflexivity|vm_compute;reflexivity]]].
 
 
 
@@ -625,9 +553,9 @@ Qed.
 
 
 #[local] Hint Resolve aux3 aux4 aux4' aux2 aux6 aux8 aux9 aux9' aux9's
-  aux10 aux11 aux12 aux7 aux5 aux13 aux16 aux15
-  aux18 aux18s aux19 aux17 aux10' aux10's aux21
-  aux15s aux4's aux20 aux10'r aux22 aux14 : proof.
+ aux10 aux11 aux12 aux7 aux5 aux13 aux16 aux15
+ aux18 aux18s aux19 aux17 aux10' aux10's aux21
+ aux15s aux4's aux20 aux10'r aux22 aux14 : proof.
 
 
 Lemma aux23 : no_proof_for ({(B ⊸ S) & (B ⊸ R), G, (G ⊸ B) ⊕ (G ⊸ S)}) R.
@@ -722,15 +650,11 @@ Qed.
 Lemma final: all_proofs_of ({ G,((B⊸S)&(B⊸R))&1,(G⊸B)⊕(G⊸S)}) (S⊕R).
 Proof.
   intros p; one_step p.
-
   apply aux1.
-
   rewrite aux27.
-  destruct (exists_AtheseA_on_formula
-         (λ (e1 : env) (f1 : formula) (_ : e1 ⊢ f1), trueP)
-         S R ({G ⊸ B, G, ((B ⊸ S) & (B ⊸ R)) & 1})
-         (S ⊕ R) i1
-    ); reflexivity.
+  match goal with
+    |- orP ?X _ = _ => destruct X ; reflexivity
+  end.
 Qed.
 
 
