ILL_equiv.v
@@ -4,37 +4,39 @@ Import ILLVarInt.MILL. (* only this *)
 Import FormulaMultiSet. (* and this *)
 Require Import narrative.
 
+Reserved Notation "x '≡≡' y" (at level 70, no associativity).
+
 Module Proof_eq.
 
 (* Implicit Types Γ Δ : env. *)
 (* Implicit Types f φ p q : formula. *)
   Set Implicit Arguments.
 
-  Inductive eq: ∀ Γ Γ' f, (Γ ⊢ f) → (Γ' ⊢ f) → Prop := 
-  | EQId: ∀ Γ1 Γ2, ∀ f, ∀ heq heq', eq (Id Γ1 f heq) (Id Γ2 f heq')
-  | EQImpl_R: ∀ Γ1 Γ2 p q h h',  eq h h' → eq (Impl_R Γ1 p q h) (Impl_R Γ2 p q h')
-  | EQImpl_L: ∀ Γ1 Δ1 Δ1' Γ2 Δ2 Δ2', ∀ p q r, ∀ heq1 heq1' heq2 heq2' h1 h1' h2 h2',
-    eq h1 h1' → eq h2 h2'
-    → eq (Impl_L Γ1 Δ1 Δ1' p q r heq1 heq2 h1 h2) (Impl_L Γ2 Δ2 Δ2' p q r heq1' heq2' h1' h2')
+  Inductive eq: ∀ {Γ Γ' f}, (Γ ⊢ f) → (Γ' ⊢ f) → Prop := 
+  | EQId: ∀ Γ1 Γ2 f heq heq', Id Γ1 f heq ≡≡ Id Γ2 f heq'
+  | EQImpl_R: ∀ Γ1 Γ2 p q h h', h ≡≡ h' → Impl_R Γ1 p q h ≡≡ Impl_R Γ2 p q h'
+  | EQImpl_L: ∀ Γ1 Δ1 Δ1' Γ2 Δ2 Δ2' p q r heq1 heq1' heq2 heq2' h1 h1' h2 h2',
+      h1 ≡≡ h1' → h2 ≡≡ h2' → (Impl_L Γ1 Δ1 Δ1' p q r heq1 heq2 h1 h2) ≡≡ (Impl_L Γ2 Δ2 Δ2' p q r heq1' heq2' h1' h2')
   | EQTimes_R: ∀ Γ1 Δ1 Δ1' Γ2 Δ2 Δ2' p q heq heq' h1 h1' h2 h2',
-    eq h1 h1' → eq h2 h2' → eq (Times_R Γ1 Δ1 Δ1' p q heq h1 h2) (Times_R Γ2 Δ2 Δ2' p q heq' h1' h2')
-  | EQTimes_L: ∀ Γ1 Γ2, ∀ p q r, ∀ hin hin' h h', eq h h' →
-    eq (Times_L Γ1 p q r hin h) (Times_L Γ2 p q r hin' h')
-  | EQOne_R: ∀ Γ1 Γ2, ∀ heq heq', eq (One_R Γ1 heq) (One_R Γ2 heq')
-  | EQOne_L: ∀ Γ1 Γ2, ∀ p, ∀ hin hin' h h', eq h h' → eq (One_L Γ1 p hin h) (One_L Γ2 p hin' h')
-  | EQAnd_R: ∀ Γ1 Γ2, ∀ p q, ∀ h1 h1' h2 h2', eq h1 h1' → eq h2 h2' → eq (And_R  Γ1 p q h1 h2) (And_R  Γ2 p q h1' h2') 
-  | EQAnd_L_2: ∀ Γ1 Γ2 p q r hin hin' h h', eq h h' → eq (And_L_2 Γ1 p q r hin h) (And_L_2 Γ2 p q r hin' h')
-  | EQAnd_L_1: ∀ Γ1 Γ2 p q r hin hin' h h', eq h h' → eq (And_L_1 Γ1 p q r hin h) (And_L_1 Γ2 p q r hin' h')
-  | EQOplus_L: ∀ Γ1 Γ2 p q r hin hin' h1 h1' h2 h2', eq h1 h1' → eq h2 h2' → eq (Oplus_L Γ1 p q r hin h1 h2) (Oplus_L Γ2 p q r hin' h1' h2')
-  | EQOplus_R_2: ∀ Γ1 Γ2 p q h h', eq h h'  → eq (Oplus_R_2 Γ1 p q h) (Oplus_R_2 Γ2 p q h')
-  | EQOplus_R_1: ∀ Γ1 Γ2 p q h h', eq h h' → eq (Oplus_R_1 Γ1 p q h) (Oplus_R_1 Γ2 p q h')
-  | EQT_ : ∀ Γ1 Γ2, eq (T_ Γ1) (T_ Γ2) (* Γ1 == Γ2 ? *)
-  | EQZero_: ∀ Γ1 Γ2 p hin hin', eq (Zero_ Γ1 p hin) (Zero_ Γ2 p hin')
-  | EQBang_D: ∀ Γ1 Γ2 p q hin hin' h h', eq h h' → eq (Bang_D Γ1 p q hin h) (Bang_D Γ2 p q hin' h')
-  | EQBang_C: ∀ Γ1 Γ2 p q hin hin' h h', eq h h' → eq (Bang_C Γ1 p q hin h) (Bang_C Γ2 p q hin' h')
-  | EQBang_W: ∀ Γ1 Γ2 p q hin hin' h h', eq h h' → eq (Bang_W Γ1 p q hin h) (Bang_W Γ2 p q hin' h')
+      h1 ≡≡ h1' → h2 ≡≡ h2' → (Times_R Γ1 Δ1 Δ1' p q heq h1 h2) ≡≡ (Times_R Γ2 Δ2 Δ2' p q heq' h1' h2')
+  | EQTimes_L: ∀ Γ1 Γ2 p q r hin hin' h h', h ≡≡ h' → (Times_L Γ1 p q r hin h) ≡≡ (Times_L Γ2 p q r hin' h')
+  | EQOne_R: ∀ Γ1 Γ2 heq heq', (One_R Γ1 heq) ≡≡ (One_R Γ2 heq')
+  | EQOne_L: ∀ Γ1 Γ2, ∀ p, ∀ hin hin' h h', h ≡≡ h' → (One_L Γ1 p hin h) ≡≡ (One_L Γ2 p hin' h')
+  | EQAnd_R: ∀ Γ1 Γ2, ∀ p q, ∀ h1 h1' h2 h2', h1 ≡≡ h1' → h2 ≡≡ h2' → And_R  Γ1 p q h1 h2 ≡≡ And_R  Γ2 p q h1' h2' 
+  | EQAnd_L_2: ∀ Γ1 Γ2 p q r hin hin' h h', h ≡≡ h' → And_L_2 Γ1 p q r hin h ≡≡ And_L_2 Γ2 p q r hin' h'
+  | EQAnd_L_1: ∀ Γ1 Γ2 p q r hin hin' h h', h ≡≡ h' → (And_L_1 Γ1 p q r hin h) ≡≡ (And_L_1 Γ2 p q r hin' h')
+  | EQOplus_L: ∀ Γ1 Γ2 p q r hin hin' h1 h1' h2 h2',
+      h1 ≡≡ h1' → h2 ≡≡ h2' → (Oplus_L Γ1 p q r hin h1 h2) ≡≡ (Oplus_L Γ2 p q r hin' h1' h2')
+  | EQOplus_R_2: ∀ Γ1 Γ2 p q h h', h ≡≡ h'  → (Oplus_R_2 Γ1 p q h) ≡≡ (Oplus_R_2 Γ2 p q h')
+  | EQOplus_R_1: ∀ Γ1 Γ2 p q h h', h ≡≡ h' → (Oplus_R_1 Γ1 p q h) ≡≡ (Oplus_R_1 Γ2 p q h')
+  | EQT_ : ∀ Γ1 Γ2, (T_ Γ1) ≡≡ (T_ Γ2)
+  | EQZero_: ∀ Γ1 Γ2 p hin hin', (Zero_ Γ1 p hin) ≡≡ (Zero_ Γ2 p hin')
+  | EQBang_D: ∀ Γ1 Γ2 p q hin hin' h h', h ≡≡ h' → (Bang_D Γ1 p q hin h) ≡≡ (Bang_D Γ2 p q hin' h')
+  | EQBang_C: ∀ Γ1 Γ2 p q hin hin' h h', h ≡≡ h' → (Bang_C Γ1 p q hin h) ≡≡ (Bang_C Γ2 p q hin' h')
+  | EQBang_W: ∀ Γ1 Γ2 p q hin hin' h h', h ≡≡ h' → (Bang_W Γ1 p q hin h) ≡≡ (Bang_W Γ2 p q hin' h')
+  where "A '≡≡' B" := (eq A B) : ILL_scope.
+
 (* inutile si pred est compatible avec == *)
-    .
 
   Lemma refl : ∀ φ Γ (h:Γ ⊢ φ), eq h h.
   Proof.
@@ -64,8 +66,7 @@ Module nu_eq.
 
   Set Implicit Arguments.
 
-  Definition eq Γ Γ' f f' (h:Γ⊢f) (h':Γ'⊢f') : Prop  := 
-    (ν _ _ h) = (ν _ _ h').
+  Definition eq Γ Γ' f f' (h:Γ⊢f) (h':Γ'⊢f') : Prop  := (ν _ _ h) = (ν _ _ h').
 
   Lemma refl : ∀ φ Γ (h:Γ ⊢ φ), eq h h.
   Proof.
@@ -90,3 +91,5 @@ Module nu_eq.
   Qed.
 
 End nu_eq.
+
+Notation "A '≡≡' B" := (Proof_eq.eq A B) : ILL_scope.
